DeBruijnSSA/BinSyntax/Rewrite/Term/Compose.lean
@@ -2,19 +2,5 @@ import DeBruijnSSA.BinSyntax.Rewrite.Term.Eqv
 import DeBruijnSSA.BinSyntax.Rewrite.Term.Compose.Seq
 import DeBruijnSSA.BinSyntax.Rewrite.Term.Compose.Product
 import DeBruijnSSA.BinSyntax.Rewrite.Term.Compose.Sum
+import DeBruijnSSA.BinSyntax.Rewrite.Term.Compose.Completeness
 import DeBruijnSSA.BinSyntax.Typing.Term.Compose
-
-import Discretion.Utils.Quotient
-
-
-namespace BinSyntax
-
-variable [Φ: EffInstSet φ (Ty α) ε] [PartialOrder α] [SemilatticeSup ε] [OrderBot ε]
-
-namespace Term
-
--- TODO: distributor
-
--- TODO: inverse distributor
-
--- TODO: distributor is iso; this gives us the desired categorical structure! yay!
